Finish ascending_le_of_pairwise_le

MergeSort/Fin/Extras.lean
@@ -39,21 +39,21 @@ theorem Fin.add_one_sub_add_ge_of_mid_lt_of_ge
     intro a b c d h1 h2
     exact add_one_sub_add_ge_of_mid_lt_of_ge_64 h1 h2
 
-def Fin.add_one_ge_of_lt_of_ge_32
+theorem Fin.add_one_ge_of_lt_of_ge_32
     {a b c : Fin 4294967296}
     (h1 : a ≥ b)
     (h2 : a < c)
     : a + 1 ≥ b := by
   omega
 
-def Fin.add_one_ge_of_lt_of_ge_64
+theorem Fin.add_one_ge_of_lt_of_ge_64
     {a b c : Fin 18446744073709551616}
     (h1 : a ≥ b)
     (h2 : a < c)
     : a + 1 ≥ b := by
   omega
 
-def Fin.add_one_ge_of_lt_of_ge
+theorem Fin.add_one_ge_of_lt_of_ge
     {a b c : Fin (2 ^ System.Platform.numBits)}
     (h1 : a ≥ b)
     (h2 : a < c)
@@ -69,3 +69,34 @@ def Fin.add_one_ge_of_lt_of_ge
     rw [h]
     intro a b c h1 h2
     exact add_one_ge_of_lt_of_ge_64 h1 h2
+
+theorem Fin.sub_add_lt_of_and_lt_lt_32
+    {a b c d : Fin 4294967296}
+    (h1 : b ≥ c)
+    (h2 : a < c ∧ b < d)
+    : a + b - c < d := by
+  omega
+
+theorem Fin.sub_add_lt_of_and_lt_lt_64
+    {a b c d : Fin 18446744073709551616}
+    (h1 : b ≥ c)
+    (h2 : a < c ∧ b < d)
+    : a + b - c < d := by
+  omega
+
+theorem Fin.sub_add_lt_of_and_lt_lt
+    {a b c d : Fin (2 ^ System.Platform.numBits)}
+    (h1 : b ≥ c)
+    (h2 : a < c ∧ b < d)
+    : a + b - c < d := by
+  cases System.Platform.numBits_eq
+  case inl h =>
+    revert a b c d h1 h2
+    rw [h]
+    intro a b c d h1 h2
+    exact sub_add_lt_of_and_lt_lt_32 h1 h2
+  case inr h =>
+    revert a b c d h1 h2
+    rw [h]
+    intro a b c d h1 h2
+    exact sub_add_lt_of_and_lt_lt_64 h1 h2
